Sandbox.fst
@@ -1,206 +1,121 @@
 module Sandbox
- 
-open FStar.Math.Lemmas
-
-let trivial_statement = fun () -> ()
-let trivial_unary_lemma = fun x -> ()
-let trivial_binary_lemma = fun x y -> ()
-let trivial_ternary_lemma = fun x y z -> ()
-
-type predicate (#a:Type) = a -> Tot bool
-type binary_op (#a:Type) = a -> a -> Tot a
-type unary_op (#a:Type) = a -> Tot a
-type binary_relation (#a:Type) = a -> a -> Tot bool
-
-let is_symmetric (#a: Type) (rel: binary_relation #a) = forall (x y: a). (rel x y ==> rel y x)
-let is_reflexive (#a: Type) (rel: binary_relation #a) = forall (x: a). (rel x x)
-let is_transitive (#a: Type) (rel: binary_relation #a) = forall (x y z: a). (rel x y /\ rel y z) ==> rel x z
-type equivalence_relation (#a:Type) = (eq:binary_relation #a{is_symmetric eq /\ is_reflexive eq /\ is_transitive eq})
-
-let associativity_condition (#a: Type) (op: binary_op #a) (eq: equivalence_relation #a) (x: a) (y: a) (z: a) = eq (op x (op y z)) (op (op x y) z)
-let commutativity_condition (#a: Type) (op: binary_op #a) (eq: equivalence_relation #a) (x: a) (y: a) = eq (op x y) (op y x)
-let neutral_element_condition (#a: Type) (op: binary_op #a) (eq: equivalence_relation #a) (neutral: a) (x: a) = eq (op neutral x) x /\ eq (op x neutral) x
-let inverse_element_condition (#a: Type) (op: binary_op #a) (inv: unary_op #a) (eq: equivalence_relation #a) (neutral: a) (x: a) 
-  = eq (op (inv x) x) neutral /\ eq (op x (inv x)) neutral
-
-let associativity_property (#a: Type) (op: binary_op #a) (eq: equivalence_relation #a) = forall (x y z: a). associativity_condition op eq x y z
-let commutativity_property (#a: Type) (op: binary_op #a) (eq: equivalence_relation #a) = forall (x y: a). commutativity_condition op eq x y
-let neutral_element_property (#a: Type) (op: binary_op #a) (eq: equivalence_relation #a) (neutral: a) = forall (x: a). neutral_element_condition op eq neutral x
-
-type neutral_element_for (#a: Type) (op: binary_op #a) (eq: equivalence_relation #a) = (x:a{neutral_element_property op eq x})
-let inverse_operation_property (#a: Type) (op: binary_op #a) (inv: unary_op #a) (eq: equivalence_relation #a) (neutral: neutral_element_for op eq) = forall (x:a). inverse_element_condition op inv eq neutral x
-type inverse_operation_for (#a: Type) (op: binary_op #a) (eq: equivalence_relation #a) (neutral: neutral_element_for op eq) = (inv: unary_op #a { inverse_operation_property op inv eq neutral })
-
-type commutativity_lemma  (#a: Type) (op: binary_op #a) (eq: equivalence_relation #a) = (x:a) -> (y:a) -> Lemma(commutativity_condition op eq x y)
-type associativity_lemma (#a: Type) (op: binary_op #a) (eq: equivalence_relation #a) =  (x:a) -> (y:a) -> (z:a) -> Lemma(associativity_condition op eq x y z)
-type element_neutrality_lemma (#a: Type) (op: binary_op #a) (eq: equivalence_relation #a) (neutral: a) = (x:a) -> Lemma(neutral_element_condition op eq neutral x)
-type inverse_lemma (#a: Type) (op: binary_op #a) (inv: unary_op #a) (eq: equivalence_relation #a) (neutral: a) = (x:a) -> Lemma(inverse_element_condition op inv eq neutral x)
-
-let neutral_uniqueness_lemma (#a: Type) (op: binary_op #a) (eq: equivalence_relation #a) (x: neutral_element_for op eq) (y: neutral_element_for op eq) : Lemma (eq x y) = ()
-
-noeq type magma (#a: Type) = { op: binary_op #a; eq: equivalence_relation #a }
-
-let op_of (#a: Type) (m: magma #a) = m.op
-let eq_of (#a: Type) (m: magma #a) = m.eq
-
-class semigroup_class (#a: Type) (sg: magma #a) = { op_is_associative: associativity_lemma sg.op sg.eq }
-class commutative_magma_class (#a: Type) (sg: magma #a) = { op_is_commutative: commutativity_lemma sg.op sg.eq }
-class monoid_class (#a: Type) (sg: magma #a)  = { is_semigroup: semigroup_class sg; neutral: neutral_element_for sg.op sg.eq; }
-
-let neutral_of (#a: Type) (m: magma #a) {| mon: monoid_class m |} = mon.neutral
-
-class commutative_monoid_class (#a: Type) (sg: magma #a) = { cm_is_monoid: monoid_class sg; cm_is_commutative_magma: commutative_magma_class sg }
-class group_class (#a: Type) (sg: magma #a) = { g_is_monoid: monoid_class sg; inverse: inverse_operation_for sg.op sg.eq g_is_monoid.neutral; }
-
-let inverse_of (#a: Type) (m: magma #a) {| g: group_class m |} = g.inverse
-
-
-class commutative_group_class (#a: Type) (sg: magma #a) = {  cg_is_commutative : commutative_magma_class sg; cg_is_group: group_class sg; }
-
-type triple 'a 'b 'c = { fst:'a; snd:'b; third:'c }
-type distrinct_triple 'a = (t: triple 'a 'a 'a { t.fst =!= t.snd /\ t. fst =!= t.third /\ t.snd =!= t.third })
- 
-type semigroup (#a:Type) = x:magma #a{semigroup_class x}
-type commutative_semigroup (#a: Type) = x:semigroup #a{commutative_magma_class x}
-type monoid (#a: Type) = x:semigroup #a{monoid_class x}
-type commutative_monoid (#a: Type) = x:monoid #a{commutative_magma_class x}
-type group (#a: Type) = x:monoid #a{group_class x}
-type commutative_group (#a: Type) = x:group #a{commutative_magma_class x}
-
-noeq type amon = 
- | Mkamon : (#a: Type) 
-    -> (op: binary_op #a) 
-    -> (eq: equivalence_relation #a) 
-    -> (#[Tactics.Typeclasses.tcresolve ()] mon: monoid_class (Mkmagma op eq)) 
-    -> amon
-
-noeq type agrp = 
- | Mkagrp : (#a: Type)
-    -> (op: binary_op #a) 
-    -> (eq: equivalence_relation #a) 
-    -> (#[Tactics.Typeclasses.tcresolve ()] mon: monoid_class (Mkmagma op eq)) 
-    -> (#[Tactics.Typeclasses.tcresolve ()] grp: group_class (Mkmagma op eq)) 
-    -> agrp
-
-instance ints_sg : semigroup_class (Mkmagma #int (+) (=)) = { op_is_associative = trivial_ternary_lemma }
-instance ints_mo : monoid_class (Mkmagma #int (+) (=)) = { is_semigroup = ints_sg; neutral = 0 }
-
-let ints = Mkamon (+) (=)
-let neut = (Mkamon?.mon ints).neutral
-
-let mag : magma #int = Mkmagma ints.op ints.eq
-
-let right_distributive_over (#a: Type) (eq: equivalence_relation #a) (multiplication: semigroup #a) (addition: commutative_group #a)
-  = forall (x y z: a). (eq (multiplication.op (addition.op y z) x) (addition.op (multiplication.op y x) (multiplication.op z x)))
-let left_distributive_over (#a: Type) (eq: equivalence_relation #a) (multiplication: semigroup #a) (addition: commutative_group #a)
-  = forall (x y z: a). (eq (multiplication.op x (addition.op y z)) (addition.op (multiplication.op x y) (multiplication.op x z)))
-let fully_distributive_over (#a: Type) (eq: equivalence_relation #a) (mul: semigroup #a) (add: commutative_group #a)
-  = (left_distributive_over eq mul add /\ right_distributive_over eq mul add)
-
-noeq type ring (#a: Type) = {
-  eq: equivalence_relation #a;
-  addition: (t:commutative_group #a{eq == t.eq});
-  multiplication: (m:monoid #a{eq == m.eq /\ fully_distributive_over eq m addition });
-}
-
-let zero_of (#a: Type) (r: ring #a) {| m: monoid_class r.addition |} = m.neutral
-let one_of (#a: Type) (r: ring #a) {| m: monoid_class r.multiplication |} = m.neutral
-let add_of (#a: Type) (r: ring #a) : binary_op #a = r.addition.op
-let mul_of (#a: Type) (r: ring #a) : binary_op #a = r.multiplication.op
-let is_zero_of (#a:Type) (r: ring #a) {| m: monoid_class r.addition |} (x: a) = r.eq m.neutral x
-let is_one_of (#a:Type) (r: ring #a) {| m: monoid_class r.multiplication |} (x: a) = r.eq m.neutral x
-
-let is_domain (#a: Type) (r: ring #a) {| m: monoid_class r.addition |} = 
-  forall (x y: a). (is_zero_of r (mul_of r x y)) ==> (is_zero_of r x) \/ (is_zero_of r y)
-
-
-type domain (#a: Type) = (z:(x: ring #a {monoid_class x.addition}){is_domain z})
-//type domain (#a: Type) = x: ring #a{}
-
-
-let list_cat (a: list int) (b: list int) : list int = a @ b
-let list_sg : magma #(list int) = { op = list_cat; eq = (=) }
-
-let assoc_cat_lemma (x: list int) (y: list int) (z: list int) 
-  : Lemma (x @ (y @ z) == (x @ y) @ z) 
-  = FStar.List.Tot.Properties.append_assoc x y z;  ()
-let assoc_forall_lemma = Classical.forall_intro_3 assoc_cat_lemma    
- 
-instance list_semi : semigroup_class list_sg = { op_is_associative = assoc_cat_lemma  }
-
-let list_sg_sg : semigroup #(list int) = 
-  let make_semigroup (#a: Type) (m: magma #a) {| semigroup_class m |} : semigroup #a = m in
-  make_semigroup list_sg
-
-instance trivially_proven_semigroup (#a: Type) (sg: magma #a{associativity_property sg.op}) : semigroup sg = { op_is_associative = trivial_ternary_lemma }
-instance trivially_proven_commutative (#a: Type) (sg: magma #a{commutativity_property sg.op}) : commutative_magma sg = { op_is_commutative = trivial_binary_lemma }
-instance trivially_proven_monoid (#a: Type) (sg: magma #a) {|sg_class: semigroup sg|} (neutral: a{neutral_element_property sg.op neutral}) : monoid sg = 
-{ 
-  is_semigroup = sg_class; 
-  neutral = neutral; 
-}
-instance trivially_proven_group (#a: Type) (sg: magma #a) {|m: monoid sg|} (inv: unary_op #a{inverse_operation_property sg.op inv m.neutral })
-  : group sg = { g_is_monoid = m; inverse = inv }
-
-let group_inverse (#a: Type) (sg: magma #a) {| g: group sg |} (x: a) = g.inverse x
-let neutral_of (#a: Type) (sg: magma #a) {| m: monoid sg |} : neutral_element_for sg.op = m.neutral
-
-let group_is_monoid (#a: Type) (sg: magma #a) {| g: group sg |} : Lemma (monoid sg) = ()
-
-let distributive_left (#a:Type) (op_mul:binary_op #a) (op_add:binary_op #a) =
-  forall (x y z:a). x `op_mul` (y `op_add` z) == (x `op_mul` y) `op_add` (x `op_mul` z)
-let distributive_right (#a:Type) (op_mul:binary_op #a) (op_add:binary_op #a) =
-  forall (x y z:a). (x `op_add` y) `op_mul` z == (x `op_mul` z) `op_add` (y `op_mul` z)
-let fully_distributive (#a:Type) (op_mul:binary_op #a) (op_add:binary_op #a) =
-  (distributive_left op_mul op_add) /\ (distributive_right op_mul op_add) 
-
-noeq type ring (#a: Type) = 
-{
-  addition: (x:magma #a {commutative_group x});
-  multiplication: (x: magma #a {semigroup x /\ fully_distributive x.op addition.op});
-}
-
-let ring_zero (#a: Type) (r: ring #a) {| m: monoid r.addition |} : neutral_element_for r.addition.op = m.neutral
-
-class commutative_ring (#a: Type) (r: ring #a) = 
-{
-  cr_is_commutative: commutativity_lemma r.multiplication.op
-}
-
-class domain (#a: Type) (r: ring #a{ monoid r.addition })  = 
-{ 
-  d_no_zero_divisors : (x: a) -> (y: a) -> Lemma(
-    let rz = ring_zero r in
-    (r.multiplication.op x y == rz) ==> (x == rz \/ y == rz)  
-  )   
-}
-
-
-let ints : magma #int = { op = op_Addition }
-instance i1_sg : semigroup ints = trivially_proven_semigroup ints
-instance i1_mo : monoid ints = trivially_proven_monoid ints 0
-instance i1_g : group ints = trivially_proven_group ints op_Minus
-
   
-type int_units = (p:int{p=1 \/ p=(-1)})
-let ints_mul_subgroup : magma #int_units = {
-  op = (fun (x:int_units) (y:int_units) -> x `op_Multiply` y)
+type binary_op (a:Type) = a -> a -> a
+type unary_op (a:Type) = a -> a
+type predicate (a:Type) = a -> bool
+type binary_relation (a: Type) = a -> a -> bool
+ 
+//[@@"opaque_to_smt"]
+let is_reflexive  (#a:Type) (r: binary_relation a) = forall (x:a).     x `r` x
+//[@@"opaque_to_smt"]
+let is_symmetric  (#a:Type) (r: binary_relation a) = forall (x y:a).   x `r` y == y `r` x
+//[@@"opaque_to_smt"]
+let is_transitive (#a:Type) (r: binary_relation a) = forall (x y z:a). x `r` y /\ y `r` z ==> x `r` z 
+
+type equivalence_relation (a: Type) = r:binary_relation a{is_reflexive r /\ is_symmetric r /\ is_transitive r}
+
+//[@@"opaque_to_smt"]
+let is_associative (#a:Type) (op:binary_op a) (eq: equivalence_relation a) = forall (x y z:a). ((x `op` y) `op` z) `eq` (x `op` (y `op` z))
+//[@@"opaque_to_smt"]
+let is_commutative (#a:Type) (op:binary_op a) (eq: equivalence_relation a) = forall (x y:a). (x `op` y) `eq` (y `op` x)
+ 
+//[@@"opaque_to_smt"]
+let is_idempotent (#a:Type) (r: unary_op a) (eq: equivalence_relation a)  = forall (x:a). (r x) `eq` (r (r x))
+ 
+//[@@"opaque_to_smt"]
+let equivalence_wrt_condition (#a: Type) (op: binary_op a) (eq: equivalence_relation a) = 
+  (forall (x y z:a). (x `eq` y) ==> ((x `op` z) `eq` (y `op` z))  /\ (z `op` x) `eq` (z `op` y))
+  
+type equivalence_wrt (#a: Type) (op: binary_op a) = eq:equivalence_relation a{equivalence_wrt_condition op eq}
+
+//[@@"opaque_to_smt"]
+let is_left_id_of  (#a:Type) (u:a) (op:binary_op a) (eq: equivalence_relation a) = forall (x:a). (u `op` x) `eq` x // left identity
+//[@@"opaque_to_smt"]
+let is_right_id_of (#a:Type) (u:a) (op:binary_op a) (eq: equivalence_relation a) = forall (x:a). (x `op` u) `eq` x // right identity
+//[@@"opaque_to_smt"]
+let is_neutral_of  (#a:Type) (u:a) (op:binary_op a) (eq: equivalence_relation a) = is_left_id_of u op eq /\ is_right_id_of u op eq // neutral element
+
+//[@@"opaque_to_smt"]
+let is_unit (#a: Type) (x: a) (op:binary_op a) (eq: equivalence_relation a) 
+  = exists (y:a). (is_neutral_of (x `op` y) op eq /\ is_neutral_of (y `op` x) op eq)
+
+//[@@"opaque_to_smt"]  
+let respects_equivalence (#a:Type) (f: unary_op a) (eq: equivalence_relation a) = forall (x y:a). (x `eq` y) ==> (f x) `eq` (f y)
+
+type units_of (#a: Type) (mul: binary_op a) (eq: equivalence_relation a) = x:a{is_unit x mul eq}
+
+//[@@"opaque_to_smt"]
+let is_inverse_operation_for (#a: Type) (inv: unary_op a) (op: binary_op a) (eq: equivalence_relation a) 
+  = (forall (x:a). is_neutral_of (op x (inv x)) op eq /\ is_neutral_of (op (inv x) x) op eq)
+
+/// The inverse operation type is also a refinement for arbitrary unary operation 
+type inverse_op_for (#a: Type) (op: binary_op a) (eq: equivalence_relation a) 
+  = (inv:unary_op a{is_inverse_operation_for inv op eq})
+
+
+type unary_op_on_units_of (#a:Type) (op: binary_op a) (eq: equivalence_wrt op) =
+  f:unary_op(units_of op eq){
+   respects_equivalence f (    
+     reveal_opaque (`%is_reflexive) (is_reflexive #a); 
+     reveal_opaque (`%is_reflexive) (is_reflexive #(units_of op eq)); 
+     reveal_opaque (`%is_symmetric) (is_symmetric #a);   
+     reveal_opaque (`%is_symmetric) (is_symmetric #(units_of op eq));   
+     reveal_opaque (`%is_transitive) (is_transitive #a);
+     reveal_opaque (`%is_transitive) (is_transitive #(units_of op eq));
+     reveal_opaque (`%is_unit) (is_unit #a);
+     eq
+   )
+  }
+
+let yields_inverses_for_units (#a:Type) (op: binary_op a) (eq: (t: equivalence_wrt op {is_associative op t})) (inv: unary_op_on_units_of op eq) = 
+  forall (x: units_of op eq). is_neutral_of (op (inv x) x) op eq /\ is_neutral_of (op x (inv x)) op eq
+
+type partial_inverse_op_for (#a:Type) (op: binary_op a) (eq: (t: equivalence_wrt op {is_associative op t})) = (f: unary_op_on_units_of op eq{yields_inverses_for_units op eq f})
+
+let inverse_is_unique (#a:Type) (op: binary_op a) 
+                                (eq: (t: equivalence_wrt op {is_associative op t})) 
+                                (inv: partial_inverse_op_for op eq)
+                                (x inv1 inv2: a) : Lemma
+                                (requires is_neutral_of (inv1 `op` x) op eq 
+                                        /\ is_neutral_of (x `op` inv1) op eq 
+                                        /\ is_neutral_of (inv2 `op` x) op eq
+                                        /\ is_neutral_of (x `op` inv2) op eq)
+                                (ensures (eq inv1 inv2 /\ eq inv2 inv1)) = admit()
+                            
+let unit_inverse_is_unit (#a:Type) (op: binary_op a) 
+                                   (eq: (t: equivalence_wrt op {is_associative op t}))
+                                   (inv: partial_inverse_op_for op eq)
+                                   (x: units_of op eq)
+                                   : Lemma (is_unit (inv x) op eq) = reveal_opaque (`%is_unit) (is_unit #a)
+
+let all_are_units (#a:Type) (op: binary_op a) (eq: equivalence_wrt op {is_associative op eq}) = 
+  forall (x:a). is_unit x op eq
+  
+noeq type magma (#a: Type) =  
+{
+  op: binary_op a;
+  eq: equivalence_wrt op;
+  inv: unary_op_on_units_of op eq;
+  neutral: a
 }
 
-let ints_mul : magma #int = { op = (fun x y -> x `op_Multiply` y) }
+let magma_inv_respects_eq (#a:Type) (m: magma #a) : Lemma (  
+  reveal_opaque (`%is_reflexive) (is_reflexive #a); 
+  reveal_opaque (`%is_reflexive) (is_reflexive #(units_of m.op m.eq)); 
+  reveal_opaque (`%is_symmetric) (is_symmetric #a);   
+  reveal_opaque (`%is_symmetric) (is_symmetric #(units_of m.op m.eq));   
+  reveal_opaque (`%is_transitive) (is_transitive #a);
+  reveal_opaque (`%is_transitive) (is_transitive #(units_of m.op m.eq));
+  reveal_opaque (`%is_unit) (is_unit #a);
+  respects_equivalence #(units_of m.op m.eq) m.inv m.eq) = ()
 
-type vertex = {
-  x: int;
-  y: int
-}
+type semigroup (#a:Type)             = g: magma #a{is_associative g.op g.eq /\ yields_inverses_for_units #a g.op g.eq g.inv}
+type commutative_magma (#a:Type)     = g: magma #a{is_commutative g.op g.eq}
+type commutative_semigroup (#a:Type) = g: semigroup #a{is_commutative g.op g.eq}
+type monoid (#a:Type)                = g: semigroup #a{is_neutral_of g.neutral g.op g.eq}
+type commutative_monoid (#a:Type)    = g: monoid #a{is_commutative g.op g.eq}
+type group (#a:Type)                 = g: monoid #a{all_are_units g.op g.eq}
+type commutative_group (#a:Type)     = g: group #a{is_commutative g.op g.eq}
 
-let rec insert' (x:vertex) (s: list vertex{has_unique_elem s}) : Tot (l : list vertex {has_unique_elem l}) =
- match s with
- | []        -> [x]
- | (hd :: tl) -> if x = hd then hd :: tl 
-                else
-                let _ = assert (x <> hd) in
-                let l = hd :: (insert' x tl) in
-                let _ = assert (has_unique_elem tl) in
-                let _ = assert (has_unique_elem l) in
-                l
+let g_inv_as_full_inv (#a:Type) (g: group #a) : inverse_op_for g.op g.eq = 
+  g.inv
